Rm cx exp

src/dynamics.lean
@@ -5,17 +5,14 @@ inductive val: exp -> Prop
 | true: val exp.true
 | false: val exp.false
 
-inductive steps: cx exp -> exp -> cx exp -> exp -> Prop
+inductive steps: exp -> exp -> Prop
 | if_e1
-    (Δ: cx exp) (Δ': cx exp)
     (e1: exp) (e1': exp) (e2: exp) (e3: exp):
-    steps Δ e1 Δ' e1' ->
-    steps Δ (exp.if_ e1 e2 e3) Δ' (exp.if_ e1' e2 e3)
+    steps e1 e1' ->
+    steps (exp.if_ e1 e2 e3) (exp.if_ e1' e2 e3)
 | if_true
-    (Δ: cx exp)
     (e2: exp) (e3: exp):
-    steps Δ (exp.if_ exp.true e2 e3) Δ e2
+    steps (exp.if_ exp.true e2 e3) e2
 | if_false
-    (Δ: cx exp)
     (e2: exp) (e3: exp):
-    steps Δ (exp.if_ exp.false e2 e3) Δ e3
+    steps (exp.if_ exp.false e2 e3) e3
